compile.bat
@@ -1,6 +1,6 @@
 coqc Basic.v
 coqc Common.v
-coqc MC.v
+coqc CC.v
 coqc Kleene.v
 coqc Implementation.v
 coqc SP.v
